 [Unit 1 - Pure Maths 1](./index.md)

# Proof and Mathematical Communication

[HOME](../index.md) | [BACK](./index.md)

***

### Mathematical structures and arguments

What's the difference between

$3x + 5 = 11$

and 

$2x + 5 = 2(x + 1 )+3$  

?

Workings...

$3x = 6$

$x = 2$

$2x + 5 = 2(x + 1 )+3$  
$2x + 5 = 2x + 2 + 3$  
$2x + 5 = 2x + 5$  
$0= 0$  

This is statement is called an **identity**
- Both left (LHS) and right (RHS) side of the statement are the same. 
- An identity is true for all values of the unknown.

**Equation** > 

$3x + 5 = 11$


**Idenity** > 

$2x + 5 = 2(x +1) + 3$

"is identically equal to" (symbol $\equiv$): 

$2x + 5 \equiv 2(x +1) + 3$


#### Example: 
In algebra $x^2 - 9$ this a **difference of two squares**

$x^2 - 9 \equiv (x -3)(x + 3)$

#### Equating coefficients in an identity: 

We can the use the method of **equating coefficients** in an identity to write a given expression in another form

To do this, match the coefficients of each variable on the lef-hand side (LHS) of the $\equiv$ symbol with the corresponding coefficient on the right-hand side (RHS)

Example : 

Here is a quadratic example 

$2x^2 + 12x - 3 \equiv a(x + p)^2 + q $

*Find the values of a,p and q ?*

Workings > 

*Multiple out the brackets to allow coefficients to be compared ?*

|                   |                                  |
| -------------     | -------------                    |
| $2x^2 + 12x -3 $  | $\equiv a(x +p)^2 + q$           |
|                   | $ = a(x^2 + 2xp + p^2) + q$      |
|                   | $ = ax^2 + 2apx + ap^2 + q$      |

*Compare coefficients*

|                   |                                  |
| -------------     | -------------                    |
|1. Coefficient of $x^2$ : | $2 = a$           |
|2. Coefficient of $x$ : | $12 = 2ap$           |
|3. Constant term  : | $-3 = ap^2 + q$           |
|                    | $ap^2 + q = -3 $           |

(Constant term is any term that doesn't have an X in it)

*Substitute $a =2 $ into the second equation*

$2 (2p) = 12$

$4p = 12$

$p = 3$

*Substitute $a =2, p = 3$ into the third equation*

2 x $3^2 + q = -3 $ 

$18 + q = -3 $ 

$q = -21 $ 

### Inequality notation

### Function notation

### Disproof by counter example

### Proof by deduction

### Proof by exhaustion


